proof/security/acai/XMSS_TW.ec
@@ -11,7 +11,6 @@ require (*--*) DigitalSignatures DigitalSignaturesROM KeyedHashFunctions HashThe
 (*---*) import SA WTW FLXMSSTW_EUFRMA.
 
 
-
 (* --- Parameters --- *)
 (* -- Proof-specific -- *)
 (* Number of allowed signature queries *)
@@ -83,6 +82,7 @@ op [lossless full uniform] dmkey : mkey distr.
 op mkg : mseed -> index -> mkey.
 
 
+theory Original.
 (* -- Proof-specific -- *)
 (* Hash-then-sign proof technique *)
 clone import HashThenSign as HtS with
@@ -412,7 +412,17 @@ qed.
 
 end section Proofs_EUF_CMA_RO_XMSSTW.
 
-(*
+end Original.
+
+
+(* Specification closer aligned with the RFC *)
+theory RFC.
+(*---*) import SA.RFC FMap.
+
+type pkXMSSTWRFC = pkFLXMSSTWRFC.
+type skXMSSTWRFC = mseed * skFLXMSSTWRFC.
+(* type msgXMSSTWRFC = msgXMSSTW. *)
+(* type sigXMSSTWRFC = sigXMSSTW. *)
 
 (* TODO: Change sk type and keygen to contain root
   perhaps change this in original proof and adjust paper, seems
@@ -420,14 +430,14 @@ end section Proofs_EUF_CMA_RO_XMSSTW.
   Also, perhaps remove address from XMSS_TW/FL_XMSS_TW_SA keys, don't seem
   to be necessary (and not in standard). Correspondingly adjust paper.
 *)
-*)
-clone import DigitalSignaturesROM as DSS_MKEY with
-  type pk_t <- pkXMSSTW,
-  type sk_t <- skXMSSTW,
+
+clone import DigitalSignaturesROM as DSS_RFC with
+  type pk_t <- pkXMSSTWRFC,
+  type sk_t <- skXMSSTWRFC,
   type msg_t <- msgXMSSTW,
   type sig_t <- sigXMSSTW,
 
-  type in_t <- (mkey * dgstblock * index) * msgXMSSTW,
+  type in_t <- mkey * (dgstblock * index * msgXMSSTW),
   type out_t <- msgFLXMSSTW,
   type d_in_t <- unit,
   type d_out_t <- bool,
@@ -435,23 +445,24 @@ clone import DigitalSignaturesROM as DSS_MKEY with
   op doutm <- fun _ => dmsgFLXMSSTW
 proof *.
 
-module XMSS_TW_MKEY (RO : DSS_MKEY.RO.POracle) = {
-    proc keygen() : pkXMSSTW * skXMSSTW = {
+
+module (XMSS_TW_RFC : DSS_RFC.KeyUpdatingROM.Scheme_RO) (RO : DSS_RFC.RO.POracle) = {
+  proc keygen() : pkXMSSTWRFC * skXMSSTWRFC = {
     var ms : mseed;
-    var pk : pkXMSSTW;
-    var skfl : skFLXMSSTW;
-    var sk : skXMSSTW;
+    var pk : pkXMSSTWRFC;
+    var skfl : skFLXMSSTWRFC;
+    var sk : skXMSSTWRFC;
 
     ms <$ dmseed;
-    (pk, skfl) <@ FL_XMSS_TW.keygen();
+    (pk, skfl) <@ FL_XMSS_TW_RFC.keygen();
     sk <- (ms, skfl);
 
     return (pk, sk);
   }
 
-  proc sign(sk : skXMSSTW, m : msgXMSSTW) : sigXMSSTW * skXMSSTW = {
+  proc sign(sk : skXMSSTWRFC, m : msgXMSSTW) : sigXMSSTW * skXMSSTWRFC = {
     var ms : mseed;
-    var skfl : skFLXMSSTW;
+    var skfl : skFLXMSSTWRFC;
     var idx : index;
     var root : dgstblock;
     var mk : mkey;
@@ -462,17 +473,18 @@ module XMSS_TW_MKEY (RO : DSS_MKEY.RO.POracle) = {
     ms <- sk.`1;
     skfl <- sk.`2;
     idx <- skfl.`1;
-    root <- witness; (* TODO: Actually compute root here, or adjust sk to contain root as well :) *)
-    mk <- Top.mkg ms idx;
-    cm <@ RO.o((mk, root, idx), m);
-    (sigfl, skfl) <@ FL_XMSS_TW.sign(skfl, cm);
+    root <- skfl.`3.`1;
+    mk <- mkg ms idx;
+    (* TODO: cm <@ RO.o((mk, root, idx), m); *)
+    cm <@ RO.o(mk, (root, idx, m));
+    (sigfl, skfl) <@ FL_XMSS_TW_RFC.sign(skfl, cm);
     sig <- (mk, sigfl);
     sk <- (ms, skfl);
 
     return (sig, sk);
   }
 
-  proc verify(pk : pkXMSSTW, m : msgXMSSTW, sig : sigXMSSTW) : bool = {
+  proc verify(pk : pkXMSSTWRFC, m : msgXMSSTW, sig : sigXMSSTW) : bool = {
     var mk : mkey;
     var sigfl : sigFLXMSSTW;
     var idx : index;
@@ -484,9 +496,376 @@ module XMSS_TW_MKEY (RO : DSS_MKEY.RO.POracle) = {
     mk <- sig.`1;
     sigfl <- sig.`2;
     idx <- sigfl.`1;
-    cm <@ RO.o((mk, root, idx), m);
-    ver <@ FL_XMSS_TW.verify(pk, cm, sigfl);
+    (* TODO: cm <@ RO.o((mk, root, idx), m); *)
+    cm <@ RO.o(mk, (root, idx, m));
+    ver <@ FL_XMSS_TW_RFC.verify(pk, cm, sigfl);
 
     return ver;
   }
 }.
+
+clone FinType as IndexFT with
+  type t <= index,
+  op enum <= map Index.insubd (range 0 l)
+
+proof *.
+realize enum_spec.
+move=> x. rewrite count_map /preim.
+admit.
+qed.
+
+clone FinProdType as DBIDX with
+  type t1 <= dgstblock,
+  type t2 <= index,
+
+  theory FT1 <= DigestBlockFT,
+  theory FT2 <= IndexFT
+
+proof *.
+
+clone FinProdType as DBIDXMSGNested with
+  type t1 <= dgstblock * index,
+  type t2 <= msgXMSSTW,
+
+  theory FT1 <= DBIDX,
+  theory FT2 <= MsgXMSSTW
+
+proof *.
+
+clone FinType as DBIDXMSG with
+  type t <= dgstblock * index * msgXMSSTW,
+  op enum <= map (fun (dbim : (_ * _) * _) => (dbim.`1.`1, dbim.`1.`2, dbim.`2)) DBIDXMSGNested.enum
+
+proof *.
+realize enum_spec.
+admit.
+qed.
+
+(* -- Proof-specific -- *)
+(* Hash-then-sign proof technique *)
+clone import HashThenSign as HtS with
+  type pk_fl_t <= pkFLXMSSTWRFC,
+  type sk_fl_t <= skFLXMSSTWRFC,
+  type msg_fl_t <= msgFLXMSSTW,
+  type sig_fl_t <= sigFLXMSSTW,
+  type rco_t <= mkey,
+  type msg_al_t <= dgstblock * index * msgXMSSTW,
+  type WithPRF.ms_t <= mseed,
+  type WithPRF.id_t <= index,
+
+    op n <- l,
+    op qS <- qS,
+    op qH <- qH,
+
+    op WithPRF.mkg <= mkg,
+    op WithPRF.extr_id <= fun (skfl : skFLXMSSTWRFC) => skfl.`1,
+
+    op dmsg_fl <= dmsgFLXMSSTW,
+    op drco <= dmkey,
+    op WithPRF.dms <= dmseed,
+
+  theory RCO <= MKey,
+  theory MSG_AL <= DBIDXMSG
+
+  proof *.
+  realize ge0_n by smt(ge2_l).
+  realize rng_qS by exact: rng_qS.
+  realize ge0_qH by exact: ge0_qH.
+  realize dmsg_fl_ll by exact: dmsgFLXMSSTW_ll.
+  realize dmsg_fl_uni by exact: dmsgFLXMSSTW_uni.
+  realize dmsg_fl_fu by exact: dmsgFLXMSSTW_fu.
+  realize drco_ll by exact: dmkey_ll.
+  realize drco_uni by exact: dmkey_uni.
+  realize drco_fu by exact: dmkey_fu.
+  realize WithPRF.dms_ll by exact: dmseed_ll.
+
+import Repro MCORO MCOROLE.
+import EUFRMAEqv DSS_FL DSS_FL_EUFRMA.
+import WithPRF MKG MKG_PRF DSS_AL_PRF KeyUpdatingROM DSS KeyUpdating.
+import WS.
+module (R_PRF_EUFCMAROXMSSTWRFC (A : Adv_EUFCMA_RO) : Adv_PRF) (O : Oracle_PRF) = {
+  module O_CMA_R_PRF_EUFCMAROXMSSTWRFC : SOracle_CMA = {
+    include var O_Base_Default
+
+    var skfl : skFLXMSSTWRFC
+
+    proc init(skfl_init : skFLXMSSTWRFC) = {
+      skfl <- skfl_init;
+      qs <- [];
+    }
+
+    proc sign(dbim : dgstblock * index * msgXMSSTW) : sigXMSSTW = {
+      var idx : index;
+      var mk : mkey;
+      var cm : msgFLXMSSTW;
+      var sigfl : sigFLXMSSTW;
+      var sig : sigXMSSTW;
+
+      idx <- skfl.`1;
+
+      mk <@ O.query(idx);
+
+      cm <@ MCO.o(mk, dbim);
+
+      (sigfl, skfl) <@ FL_XMSS_TW_RFC.sign(skfl, cm);
+
+      sig <- (mk, sigfl);
+
+      return sig;
+    }
+  }
+
+  proc distinguish() : bool = {
+    var pk : pkXMSSTWRFC;
+    var skfl : skFLXMSSTWRFC;
+    var dbim : dgstblock * index * msgXMSSTW;
+    var sig : sigXMSSTW;
+    var is_valid, is_fresh;
+
+    MCO.init();
+
+    (pk, skfl) <@ FL_XMSS_TW_RFC.keygen();
+
+    O_CMA_R_PRF_EUFCMAROXMSSTWRFC.init(skfl);
+
+    (dbim, sig) <@ A(MCO, O_CMA_R_PRF_EUFCMAROXMSSTWRFC).forge(pk);
+
+    is_valid <@ XMSS_TW_RFC(MCO).verify(pk, dbim.`3, sig);
+
+    is_fresh <@ O_CMA_R_PRF_EUFCMAROXMSSTWRFC.fresh(dbim);
+
+    return is_valid /\ is_fresh;
+  }
+}.
+
+
+(* --- Proofs of EUF-CMA property for XMSS-TW (assuming message compression is a RO) --- *)
+section Proofs_EUF_CMA_RO_XMSSTW.
+(* -- Declarations -- *)
+(* Models the signing procedure of FL-XMSS-TW *)
+declare op opsign : skFLXMSSTW -> msgFLXMSSTW -> sigFLXMSSTW * skFLXMSSTW.
+
+(* opsign precisely captures the semantics of the signing procedure of FL-XMSS-TW *)
+declare axiom FLXMSSTW_sign_fun (skfl : skFLXMSSTW) (cm : msgFLXMSSTW) :
+  hoare[FL_XMSS_TW.sign: arg = (skfl, cm) ==> res = opsign skfl cm].
+
+(* The signing procedure of FL-XMSS-TW is lossless (and captured by opsign) *)
+local lemma FLXMSSTW_sign_pfun (skfl : skFLXMSSTW) (cm : msgFLXMSSTW) :
+  phoare[FL_XMSS_TW.sign: arg = (skfl, cm) ==> res = opsign skfl cm] = 1%r.
+proof. by conseq FLXMSSTW_sign_ll (FLXMSSTW_sign_fun skfl cm). qed.
+
+(* Adversary against EUF-CMA in the ROM *)
+declare module A <: Adv_EUFCMA_RO{-FL_XMSS_TW, -ERO, -O_CMA_Default, -O_METCR, -R_EUFCMARO_CRRO, -R_EUFCMARO_METCRRO, -Repro.Wrapped_Oracle, -Repro.RepO, -O_RMA_Default, -R_EUFCMARO_IEUFRMA, -QC_A, -Lazy.LRO, -Repro.ReproGame, -R_EUFRMA_IEUFRMA, -R_PRF_EUFCMARO, -O_PRF_Default, -DSS_AL.DSS.KeyUpdating.O_CMA_Default, -PRF_SK_PRF.O_PRF_Default, -FC.O_THFC_Default, -FC_PRE.O_SMDTPRE_Default, -FC_TCR.O_SMDTTCR_Default, -FC_UD.O_SMDTUD_Default, -O_MEUFGCMA_WOTSTWES, -PKCOC.O_THFC_Default, -PKCOC_TCR.O_SMDTTCR_Default, -TRHC.O_THFC_Default, -TRHC_TCR.O_SMDTTCR_Default, -R_SMDTUDC_Game23WOTSTWES, -R_SMDTTCRC_Game34WOTSTWES, -R_PRF_FLXMSSTWESInlineNOPRF, -R_SMDTPREC_Game4WOTSTWES, -R_MEUFGCMAWOTSTWES_EUFRMAFLXMSSTWESNOPRF, -R_SMDTTCRCTRH_EUFRMAFLXMSSTWESNOPRF, -R_SMDTTCRCPKCO_EUFRMAFLXMSSTWESNOPRF, -R_SMDTTCRCTRH_EUFRMAFLXMSSTWESNOPRF, -R_EUFRMAFLXMSSTW_EUFRMAFLXMSSTWES}.
+
+(* The adversary always terminates if the oracle procedures it can call terminate *)
+declare axiom A_forge_ll (RO <: POracle{-A}) (SO <: SOracle_CMA{-A}) :
+  islossless RO.o => islossless SO.sign => islossless A(RO, SO).forge.
+
+(* The adversary makes a limited number of queries to the given random (hash) oracle and signing oracle *)
+declare axiom A_forge_queries (RO <: POracle{-A, -QC_A}) (SO <: SOracle_CMA{-A, -QC_A}) :
+  hoare[A(QC_A(A, RO, SO).QC_RO, QC_A(A, RO, SO).QC_SO).forge :
+    QC_A.cH = 0 /\ QC_A.cS = 0 ==> QC_A.cH <= qH /\ QC_A.cS <= qS].
+
+
+(* -- Security theorems -- *)
+(*
+  High-level security theorem (based on EUF-RMA of FL-XMSS-TW):
+  XMSS-TW is EUF-CMA secure in the ROM if mkg (i.e., the function that generates
+  indexing keys for the message compression function) is a PRF, MCO (i.e., the message
+  compression function) is a collision-resistant random oracle, and FL-XMSS-TW is EUF-RMA
+  secure
+*)
+lemma EUFCMARO_XMSSTW_EUFRMA &m :
+  Pr[EUF_CMA_RO(XMSS_TW, A, O_CMA_Default, MCO).main() @ &m : res]
+  <=
+  `| Pr[PRF(R_PRF_EUFCMARO(FL_XMSS_TW, A), O_PRF_Default).main(false) @ &m : res] -
+     Pr[PRF(R_PRF_EUFCMARO(FL_XMSS_TW, A), O_PRF_Default).main(true) @ &m : res] |
+  +
+  Pr[CR_RO(R_EUFCMARO_CRRO(FL_XMSS_TW, A), MCO).main() @ &m : res]
+  +
+  Pr[EUF_RMA(FL_XMSS_TW, R_EUFRMA_IEUFRMA(R_EUFCMARO_IEUFRMA(A))).main() @ &m : res]
+  +
+  qS%r * (qS + qH + 1)%r * mu1 dmkey witness
+  +
+  l%r * mu1 dmsgFLXMSSTW witness.
+proof.
+have ->:
+  Pr[EUF_CMA_RO(XMSS_TW, A, O_CMA_Default, MCO).main() @ &m : res]
+  =
+  Pr[EUF_CMA_RO(WithPRF.AL_KU_DSS(FL_XMSS_TW), A, O_CMA_Default, MCO).main() @ &m : res].
++ byequiv => //.
+  proc; inline{1} 2; inline{2} 2.
+  seq 5 5 : (={O_Base_Default.qs, m, is_valid}); last by sim.
+  inline{1} 5; inline{2} 5.
+  inline{1} 11; inline{2} 11.
+  wp; call(: true) => />; 1: by sim.
+  wp; call(: ={ERO.m}) => />; 1: by wp.
+  wp; call(: ={O_Base_Default.qs, O_CMA_Default.sk, ERO.m}) => />; first 2 by sim.
+  inline *.
+  wp; while (={ss1, ss0, ps1, ps0, ms, leafl0, ad0, ERO.m}); 1: by sim.
+  wp; do 3! rnd.
+  while (={w, ERO.m}); 1: by wp; rnd; wp; skip.
+  by wp; skip.
+move: (ALKUDSS_EUFCMARO_PRF_CRRO_EUFRMA FL_XMSS_TW FLXMSSTW_sign_ll FLXMSSTW_verify_ll).
+move=> /(_ (fun (skfl : skFLXMSSTW) => skfl.`1 = Index.insubd 0)
+           (fun (skfl : skFLXMSSTW) => (Index.insubd (Index.val skfl.`1 + 1), skfl.`2, skfl.`3, skfl.`4))
+           opsign _ FLXMSSTW_sign_fun _ _ _ _).
++ proc; inline *.
+  wp; while (true).
+  - wp; while (true); 1: by wp.
+    wp; while (true); 1: by wp.
+    by wp.
+  by wp; do 2! rnd; skip.
++ move=> skfl.
+  proc; inline *.
+  wp => />; while (true).
+  - wp; while (true); 1: by wp.
+    wp; while (true); 1: by wp.
+    by wp.
+  wp; while (true); 1: by wp.
+  wp; while (true); 1: by wp.
+  by wp; skip.
++ move=> i j skfl /= init_sk [ge0i leqS_i] [ge0_j leqS_j] neqj_i.
+  have fupd_it:
+    forall (k : int), 0 <= k => k < qS =>
+      (fold (fun (sk : skFLXMSSTW) =>
+        ((Index.insubd ((Index.val sk.`1) + 1)), sk.`2, sk.`3, sk.`4)) skfl k).`1
+      =
+      Index.insubd k.
+  - elim => [@/fupd | k ge0_k @/fupd ih ltqS_k1].
+    * by rewrite fold0.
+    rewrite foldS //= ih 2:Index.insubdK //; smt(rng_qS).
+  rewrite fupd_it // fupd_it //.
+  move: neqj_i; apply contra => eqins_ij.
+  by rewrite -(Index.insubdK i) 2:-(Index.insubdK j) 3:eqins_ij; 1,2: smt(rng_qS).
++ by sim.
++ by sim.
+by move=> /(_ A A_forge_ll A_forge_queries &m).
+qed.
+
+
+(*
+  Low-level security theorem (based on properties of KHFs and THFs)
+  XMSS-TW is EUF-CMA secure in the ROM if mkg (i.e., the function that generates
+  indexing keys for the message compression function) is a PRF; MCO (i.e., the message
+  compression function) is a collision-resistant random oracle; prf_sk (i.e., the
+  function used to generate WOTS-TW secret keys) is a PRF; f (i.e., the function used
+  in the WOTS-TW chains) has SM-DT-UD-C, SM-DT-TCR-C, and SM-DT-PRE-C; pkco (i.e., the
+  fucntion used to compress WOTS-TW public keys to leaves of the binary hash tree) has
+  SM-DT-TCR-C; and trh (i.e., the function used to construct the full binary hash tree from
+  the leaves) has SM-DT-TCR-C.
+*)
+lemma EUFCMARO_XMSSTW &m :
+  Pr[EUF_CMA_RO(XMSS_TW, A, O_CMA_Default, MCO).main() @ &m : res]
+  <=
+  `| Pr[MKG_PRF.PRF(R_PRF_EUFCMARO(FL_XMSS_TW, A), O_PRF_Default).main(false) @ &m : res] -
+     Pr[MKG_PRF.PRF(R_PRF_EUFCMARO(FL_XMSS_TW, A), O_PRF_Default).main(true) @ &m : res] |
+  +
+  Pr[CR_RO(R_EUFCMARO_CRRO(FL_XMSS_TW, A), MCO).main() @ &m : res]
+  +
+  `|Pr[PRF_SK_PRF.PRF(R_PRF_FLXMSSTWESInlineNOPRF(R_EUFRMAFLXMSSTW_EUFRMAFLXMSSTWES(R_EUFRMA_IEUFRMA(R_EUFCMARO_IEUFRMA(A)))), PRF_SK_PRF.O_PRF_Default).main(false) @ &m : res] -
+  Pr[PRF_SK_PRF.PRF(R_PRF_FLXMSSTWESInlineNOPRF(R_EUFRMAFLXMSSTW_EUFRMAFLXMSSTWES(R_EUFRMA_IEUFRMA(R_EUFCMARO_IEUFRMA(A)))), PRF_SK_PRF.O_PRF_Default).main(true) @ &m : res]|
+  +
+  (w - 2)%r *
+`|Pr[FC_UD.SM_DT_UD_C(R_SMDTUDC_Game23WOTSTWES(R_MEUFGCMAWOTSTWES_EUFRMAFLXMSSTWESNOPRF(R_EUFRMAFLXMSSTW_EUFRMAFLXMSSTWES(R_EUFRMA_IEUFRMA(R_EUFCMARO_IEUFRMA(A))))), FC_UD.O_SMDTUD_Default, FC.O_THFC_Default).main(false) @ &m : res] -
+  Pr[FC_UD.SM_DT_UD_C(R_SMDTUDC_Game23WOTSTWES(R_MEUFGCMAWOTSTWES_EUFRMAFLXMSSTWESNOPRF(R_EUFRMAFLXMSSTW_EUFRMAFLXMSSTWES(R_EUFRMA_IEUFRMA(R_EUFCMARO_IEUFRMA(A))))), FC_UD.O_SMDTUD_Default, FC.O_THFC_Default).main(true) @ &m : res]|
+  +
+  Pr[FC_TCR.SM_DT_TCR_C(R_SMDTTCRC_Game34WOTSTWES(R_MEUFGCMAWOTSTWES_EUFRMAFLXMSSTWESNOPRF(R_EUFRMAFLXMSSTW_EUFRMAFLXMSSTWES(R_EUFRMA_IEUFRMA(R_EUFCMARO_IEUFRMA(A))))), FC_TCR.O_SMDTTCR_Default, FC.O_THFC_Default).main() @ &m : res]
+  +
+  Pr[FC_PRE.SM_DT_PRE_C(R_SMDTPREC_Game4WOTSTWES(R_MEUFGCMAWOTSTWES_EUFRMAFLXMSSTWESNOPRF(R_EUFRMAFLXMSSTW_EUFRMAFLXMSSTWES(R_EUFRMA_IEUFRMA(R_EUFCMARO_IEUFRMA(A))))), FC_PRE.O_SMDTPRE_Default, FC.O_THFC_Default).main() @ &m : res]
+  +
+  Pr[PKCOC_TCR.SM_DT_TCR_C(R_SMDTTCRCPKCO_EUFRMAFLXMSSTWESNOPRF(R_EUFRMAFLXMSSTW_EUFRMAFLXMSSTWES(R_EUFRMA_IEUFRMA(R_EUFCMARO_IEUFRMA(A)))), PKCOC_TCR.O_SMDTTCR_Default, PKCOC.O_THFC_Default).main() @ &m : res]
+  +
+  Pr[TRHC_TCR.SM_DT_TCR_C(R_SMDTTCRCTRH_EUFRMAFLXMSSTWESNOPRF(R_EUFRMAFLXMSSTW_EUFRMAFLXMSSTWES(R_EUFRMA_IEUFRMA(R_EUFCMARO_IEUFRMA(A)))), TRHC_TCR.O_SMDTTCR_Default, TRHC.O_THFC_Default).main() @ &m : res]
+  +
+  qS%r * (qS + qH + 1)%r * mu1 dmkey witness
+  +
+  l%r * mu1 dmsgFLXMSSTW witness.
+proof.
+move: (EUFRMA_FLXMSSTW (R_EUFRMA_IEUFRMA(R_EUFCMARO_IEUFRMA(A))) _ &m) (EUFCMARO_XMSSTW_EUFRMA &m); last first.
+have -> /#:
+  Pr[FLXMSSTW_EUFRMA.EUF_RMA(FL_XMSS_TW, R_EUFRMA_IEUFRMA(R_EUFCMARO_IEUFRMA(A))).main() @ &m : res]
+  =
+  Pr[EUF_RMA(FL_XMSS_TW, R_EUFRMA_IEUFRMA(R_EUFCMARO_IEUFRMA(A))).main() @ &m : res].
++ by byequiv => //; sim.
+proc; inline *.
+wp; call (: true).
++ by move=> RO SO ROll SOll; apply (A_forge_ll RO SO).
++ proc; inline *.
+  wp; rnd; skip => />.
+  by apply dmkey_ll.
++ proc; inline *.
+  by wp; skip.
+wp; while (true) (size w).
++ move=> z.
+  wp; rnd; wp; skip => /> &1 neqel_w.
+  split; 2: by apply dmsgFLXMSSTW_ll.
+  by elim: (w{1}) neqel_w => //= /#.
+by wp; skip => />; smt(size_eq0 size_ge0).
+qed.
+
+(**
+  Reduction adversary reducing EUF-CMA for original specification to that of
+  RFC-like specification
+**)
+module (R_EUFCMA_XMSSTW_XMSSTWRFC (A : DSS_RFC.KeyUpdatingROM.Adv_EUFCMA_RO) : DSS_AL_PRF.KeyUpdatingROM.Adv_EUFCMA_RO)
+       (RO : DSS_AL_PRF.RO.POracle) (O : DSS_AL_PRF.DSS.KeyUpdating.SOracle_CMA) = {
+  var pkroot : dgstblock
+(*
+  module RO_R : DSS_RFC.RO.POracle = {
+    var mp : ((mkey * dgstblock * index) * msgXMSSTW, msgFLXMSSTW) fmap
+
+    proc init() : unit = {
+      mp <- empty;
+    }
+
+    proc o(rm : (mkey * dgstblock * index) * msgXMSSTW) : msgFLXMSSTW = {
+      var mk : mkey;
+      var root : dgstblock;
+      var idx : index;
+      var m : msgXMSSTW;
+      var cm : msgFLXMSSTW;
+
+      (mk, root, idx) <- rm.`1;
+      m <- rm.`2;
+      if (root = pkroot) {
+       cm <@ RO.o((mk, m));
+      } else {
+        cm <$ dmsgFLXMSSTW;
+        if (rm \notin mp) {
+          mp.[rm] <- cm;
+        }
+        cm <- oget mp.[rm];
+      }
+
+      return cm;
+    }
+  }
+*)
+
+  module O_R : DSS_RFC.DSS.KeyUpdating.SOracle_CMA = {
+    var qs : msgXMSSTW list
+
+    proc init() : unit = {
+      qs <- [];
+    }
+    proc sign(m : msgXMSSTW) : sigXMSSTW = {
+      var sig : sigXMSSTW;
+
+      qs <- rcons qs m;
+
+      return witness;
+    }
+  }
+
+  proc forge(pk : pkXMSSTW) : msgXMSSTW * sigXMSSTW = {
+    var m : msgXMSSTW;
+    var sig : sigXMSSTW;
+
+    (m, sig) <@ A(DSS_RFC.RO.Lazy.LRO, O_R).forge(pko2pkr pk);
+
+    return (m, sig);
+  }
+}.
+
+end RFC.
